layout: proof
categories: branches,number-systems-arithmetics
nodeid: bookofproofs$1408
orderid: 50
parentid: bookofproofs$1407
title: 
description:  Proof of ALTERNATING SUM OF BINOMIAL COEFFICIENTS &#9733; graduate maths &#10004; step by step &#10010; visit BookOfProofs now!
references: bookofproofs$581
keywords: alternating,binomial,coefficients,sum,alternating sum of binomial coefficients,sum of binomial coefficients,alternating sum,alternating binomial sum,sum binomial coefficients,proof
contributors: bookofproofs

---


---

The closed formula for the alternating [sum][bookofproofs$216] of [binomial coefficients][bookofproofs$993].
`\[\sum_{k=0}^n (-1)^n\binom nk=0\]` 
follows immediately from the [binomial theorem][bookofproofs$1397].
`\[\sum_{k=0}^n{n\choose k}x^{n-k}y^k=(x+y)^n\]`
by setting `\(x=1\)` and `\(y=-1\)`.
