layout: proof
categories: branches,number-systems-arithmetics
nodeid: bookofproofs$537
orderid: 50
parentid: bookofproofs$535
title: 
description: ELEMENTARY PROOF Proof of -(X+Y)=-X-Y ★ graduate maths ✔ step by step ✚ by the axiomatic method ➜ visit BookOfProofs now!
references: bookofproofs$581
keywords: real number,real numbers,proof,proof
contributors: bookofproofs

---


---

* From the [existence of the negative numbers][bookofproofs$35] it follows that `\[(x+y)+(-(x+y))=0.\]`
* Adding `\((-x)\)` to both sides of the equation results in `\[y+(-(x+y))=-x.\]`
* On the other hand, from the [unique solvability][bookofproofs$516] of the equation `\(a+x=b\)` with the solution  `\(x=b-a\)` it follows that the equation `\(y+z=-x\)` has the unique solution `\(z=-x-y\)`.
* This proofs the statement `\(-(x+y)=-x-y\)`.
