layout: proof
categories: branches,number-systems-arithmetics
nodeid: bookofproofs$532
orderid: 50
parentid: bookofproofs$530
title: 
description: ELEMENTARY PROOF Proof of \-XY=-XY\ &#9733; graduate maths &#10004; step by step &#10010; by the axiomatic method &#10140; visit BookOfProofs now!
references: bookofproofs$581
keywords: brackets,minus,outside,placed,proof
contributors: bookofproofs

---


---

* As a consequence from the [existence of negative numbers][bookofproofs$35] it follows that `$xy+(-(xy))=0.$`
* On the other hand, it follows from the [distributivity law][bookofproofs$520] and its [corollary][bookofproofs$521] `\(0x=0\)` that `$xy+(-x)y=(x+(-x))y=0y=0.$`
* Comparing both equations, the result `\((-x)y=-(xy)\)` follows as a corollary from the [uniqueness of negative numbers][bookofproofs$50].