layout: proof
categories: branches,number-systems-arithmetics
nodeid: bookofproofs$533
orderid: 50
parentid: bookofproofs$531
title: 
description: ELEMENTARY PROOF Proof of \-X-Y=XY\ &#9733; graduate maths &#10004; step by step &#10010; by the axiomatic method &#10140; visit BookOfProofs now!
references: 
keywords: equals,minus,plus,times,proof
contributors: bookofproofs

---


---

As a corollary from the [statement][bookofproofs$530] `\((-x)y=-(xy)\)` for all `\(x,y\in\mathbb R\)` the following two results follow: `\[(-x)(-y)=-(x(-y))\]`and `\[x(-y)=-(xy)\]`This means that `\((-x)(-y)=-(-(xy))\)`. With this preliminary result, and the statement `\((-x)(-y)=xy\)` follows now from the statement `\(-(-x)=x\)`, which was [proven here][bookofproofs$522].