layout: proof
categories: branches,number-systems-arithmetics
nodeid: bookofproofs$538
orderid: 50
parentid: bookofproofs$536
title: 
description: ELEMENTARY PROOF Proof of (XY)^{-1}=X^{-1}Y^{-1} ★ graduate maths ✔ step by step ✚ visit BookOfProofs now!
references: bookofproofs$581
keywords: real number,real numbers,proof,proof
contributors: bookofproofs

---


---

* From the [existence of the reciprocal numbers][bookofproofs$42] it follows that `$(xy)\cdot(xy)^{-1}=1$` for all `$x,y\in\mathbb R.$`
* Multiplying both sides of the equation by `$x^{-1}$` results in `$y\cdot(xy)^{-1}=x^{-1}.$`
* Since `$x=ba^{-1}$` is the [only unique solution][bookofproofs$517] of `$ax=b,$` it follows that the equation `$yz=x^{-1}$` has the unique solution `$z=x^{-1}y^{-1}.$` 
* This proofs the statement `$(xy)^{-1}=x^{-1}y^{-1}.$`
