layout: proof
categories: branches,analysis
nodeid: bookofproofs$1134
orderid: 50
parentid: bookofproofs$1133
title: 
description:  Proof of DIFFERENCE OF CONVERGENT REAL SEQUENCES &#9733; graduate maths &#10004; step by step &#10010; visit BookOfProofs now!
references: bookofproofs$581
keywords: difference of convergent real sequences,difference of limits,proof
contributors: bookofproofs

---


---

The proposition follows immediately from the corresponding proposition for the [sum of convergent real series][bookofproofs$1131], the [definition of subtracting real numbers][bookofproofs$1588], and the [product of a real number and a convergent real sequence][bookofproofs$1140]:

`\[\begin{array}{rcll}\lim_{n\rightarrow\infty} (a_n - b_n)&=&\lim_{n\rightarrow\infty} (a_n  + ( -  b_n))&\text{by definition of subtracting real numbers}\\
&=&\lim_{n\rightarrow\infty} a_n + \lim_{n\rightarrow\infty} ( -1 )\cdot b_n&\text{sum of convergent real series}\\
&=&\lim_{n\rightarrow\infty} a_n + (-1)\cdot\lim_{n\rightarrow\infty} b_n&\text{product of a real number and a convergent real sequence}\\
&=&\lim_{n\rightarrow\infty} a_n - \lim_{n\rightarrow\infty} b_n&\text{by definition of subtracting real numbers}.
\end{array}\]`
