layout: proof
categories: branches,analysis
nodeid: bookofproofs$1602
orderid: 50
parentid: bookofproofs$1601
title: 
description:  Proof of FUNCTIONAL EQUATION OF THE NATURAL LOGARITHM &#9733; graduate maths &#10004; step by step &#10010; visit BookOfProofs now!
references: bookofproofs$581
keywords: logarithm,natural,natural logarithm,proof,proof
contributors: bookofproofs

---


---

According to the [functional equation of the exponential function][bookofproofs$1415], we have `\[\exp(\xi+\eta)=\exp(\xi)\cdot \exp(\eta)\quad\quad ( * )\]` for all real numbers `\(\xi,\eta\in\mathbb R\)`. Because the natural logarithm `\[\ln:\mathbb R_{+}^*\to\mathbb R.\]` is its [inverse function][bookofproofs$1421], by setting `\[\begin{array}{rcl}x=\exp(\xi)&\Longleftrightarrow&\xi=\ln (x),\\
y=\exp(\eta)&\Longleftrightarrow&\eta=\ln (y),
\end{array}\]`

With these substitutions and the equation `\( ( * ) \)`, we get:
`\[\begin{array}{rcl}
\exp(\xi+\eta)&=&x\cdot y\\
\ln(\exp(\xi+\eta))&=&\ln(x\cdot y)\\
\xi+\eta&=&\ln(x\cdot y)\\
\ln (x)+\ln (y)&=&\ln(x\cdot y)
\end{array}\]`
for for all [positive real numbers][bookofproofs$1107] `\(x,y\in\mathbb R_+^*\)`. It follows that the [natural logarithm][bookofproofs$1421] fulfills the [functional equation][bookofproofs$6726] `$\ln(xy)=\ln(x) + \ln(y).$`
