layout: proof
categories: branches,algebra
nodeid: bookofproofs$816
orderid: 0
parentid: bookofproofs$815
title: 
description: PROOF OF GROUP HOMOMORPHISMS WITH CYCLIC GROUPS &#9733; graduate maths &#10004; step by step &#10010; by the axiomatic method &#10140; visit BookOfProofs now!
references: 
keywords: cyclic groups,homomorphisms,proof
contributors: bookofproofs
issues: broken-links

---


---

### "`\(\Rightarrow\)`"

Let `\((G,\ast)\)` be a "cyclic":https://www.bookofproofs.org/branches/cyclic-group/ group generated by the element `\(g\)`. We have to find a surjective group homomorphism from the set `\(\mathbb Z\)` of all integers to `\(G\)`. First, we define for all `\(k\in\mathbb Z\)` a map:
`\[f:\begin{cases}
\mathbb Z&\mapsto G \\
k&\mapsto g^k
\end{cases}\]`
For any two integers `\(k,l\in\mathbb Z\)` we then have 

`\[f(k+l)=g^{k+l}=g^k\ast g^l.\]`
It follows that `\(f\)` is a [group homomorphism][bookofproofs$679] Since the sum `\(k+l\)` can represent any integer `\(j\in\mathbb Z\)` (for a given `\(j\)`, fix `\(k\)` and set `\(l:=j-k\)`), `\(g^j\)` can generate all (even infinitely many) elements of `\(G\)`. Therefore, `\(f\)` is [surjective][bookofproofs$770]

### "`\(\Leftarrow\)`"

Let `\(f:\mathbb Z\mapsto G\)` be a [surjective][bookofproofs$770]  [group homomorphism][bookofproofs$679], i.e. 

`\[f(k+l)=f(k)\ast f(l)\in G,\]`
for any integers `\(k,l\in\mathbb Z\)` with `\(im(f)=G\)`. We have to show that `\(G\)` is cyclic. In particular, we have to prove that there exist an integer `\(j\)`, for which `\(G=\langle f(j) \rangle\)`, i.e. for which each element of `\(G\)` can be represented as some power of `\(f(j)\)`. We will show that `\(j=1\)` will do the trick. First of all, note that because `\(f\)` is a group homomorphism, we can generate all elements `\(f(k)\in G\)` with `\(k \ge 1\)` as "powers" of `\(f(1)\)` as follows:

`\[\begin{array}{ccl}
f(1)&=&f(1)^1\\ 
f(2)&=&f(1+1)=f(1)\ast f(1)=f(1)^2\\
\vdots\\
f(k)&=&f(\underbrace{1+\ldots+1}_{k\text{ times}})=\underbrace{f(1)\ast\ldots \ast f(1)}_{k\text{ times}}=f(1)^k.\\ 
\end{array}\]`

Following the [properties of group homomorphism][bookofproofs$680], also `\(f(-1)\)` can be generated from `\(f(1)\)` by the equation 

`\[f(-1)=f(1)^{-1}.\]`

Therefore, we can also generate all elements `\(f(k)\in G\)` with `\(k \le -1\)` as "powers" of `\(f(1)\)` as follows:

`\[\begin{array}{ccl}
f(-1)&=&f(1)^{-1}\\ 
f(-2)&=&f(-1-1)=f(1)^{-1}\ast f(1)^{-1}=f(1)^{-2}\\
\vdots\\
f(-k)&=&f(\underbrace{-1-\ldots-1}_{k\text{ times}})=\underbrace{f(1)^{-1}\ast\ldots \ast f(1)^{-1}}_{k\text{ times}}=f(1)^{-k}.\\ 
\end{array}\]`

Finally, again following the [properties of group homomorphism][bookofproofs$680], also the identity `\(e_G\)` of the group `\(G\)` can be generated from `\(f(1)\)` by the equation 

`\[e_G=f(0)=f(-1)\ast f(1)=f(1)^{-1}\ast f(1)^1=f(1)^0.\]` 

Because `\(f\)` is surjective and we have explored all integers `\(k\in\mathbb Z\)`, we must have generated all elements of `\(G\)` by only the element `\(f(1)\in G\)`. Thus, `\(G=\langle f(1) \rangle\)`.
